\documentclass[12pt]{reedthesis}
\usepackage{main}
\usepackage[left=1cm, right=1cm]{geometry}


\begin{document}
.\\ \vspace{2em}

% ------------------------------------------------------------------------------
% Func
% ------------------------------------------------------------------------------

% \begin{snippet}
% type boolean : kind
%   { true  : boolean
%   | false : boolean }.
%
% term natural : kind
%   { zero : natural
%   | succ : natural → natural }.
%
% term add (m n : natural) : natural
%   ≔ cases m
%       { zero    ⇒ n
%       | succ m' ⇒ succ (add m' n) }.
%
% term mul (m n : natural) : natural
%   ≔ cases m
%       { zero    ⇒ zero
%       | succ m' ⇒ add n (mul m' n) }.
%
% type list (α:kind) : kind
%   { nil : list α
%   | app : α → list α → list α }.
%
%         []   $\syneq$   nil
%
%       $a$ ∷ $l$   $\syneq$   app $a$ $l$
%
% [$a_1$, $\dots$, $a_n$]   $\syneq$   $a_1$ ∷ $\cdots$ ∷ $a_n$ ∷ []
%
% term fold : (α β : kind) ⇒ (β → α → β) → β → list α → β
%   ≔ f b l ⇒ cases l
%               { []     ⇒ b
%               | a ∷ l' ⇒ fold f (f b a) l' }
%
% term list-sum : list integer → integer ≔ fold add 0
% \end{snippet}

% ------------------------------------------------------------------------------
% Impe
% ------------------------------------------------------------------------------

% \begin{snippet}
% primitive type exception-of : kind → kind.
%
% primitive term throw    (α β : kind) : exception-of α → α → β.
% primitive term catching (α β : kind) : (exception-of α → α → β) → β → β.
%
% catch { $e$ $a$ ⇒ $b'$ } in $b$   $\syneq$   catching ($e$ $a$ ⇒ $b'$) $b$
%
% exception division-by-0 of rational.
%
% term divide-safely (r s : rational) : rational
%   ≔ if s == 0
%       then throw (division-by-0 r)
%       else r/s.
%
% catch { division-by-0 r ⇒ 0 } in
%   divide-safely 5 0
%
% term head-of-nil of unit.
%
% term head-safely (α:kind) (l : list α) : α
%   ≔ cases l
%       { []    ⇒ throw (head-of-nil •)
%       ; a ∷ _ ⇒ a }.
% \end{snippet}

% \begin{snippet}
% primitive term sample (α:kind) : list α → α.
%
% term flip-coin (_:unit) : boolean ≔ sample [true, false].
%
% term lucky (_:unit) : boolean
%   ≔ let b1 ≔ flip-coin • in
%     let b2 ≔ flip-coin • in
%     b1 ∧ b2.
%
% $\ndctx$ $\|$ lucky •
% $↠$
% $\ndctx$ $\|$ let b1 ≔ flip-coin • in
%       let b2 ≔ flip-coin • in
%       b1 ∧ b2.
% $↠$
% $\ndctx$ $\|$ let b1 ≔ $\ndctx_1$(flip-coin •) in
%       let b2 ≔ $\ndctx_2$(flip-coin •) in
%       b1 ∧ b2.
% $↠$
% $\ndctx$ $\|$ $\ndctx_1$(flip-coin •) ∧ $\ndctx_2$(flip-coin •).
% \end{snippet}

% \begin{snippet}
% primitive type mutable : kind → kind.
%
% primitive term initialize (α:kind) : α → mutable α.
% primitive term get        (α:kind) : mutable α → α.
% primitive term set        (α:kind) : mutable α → α → unit.
%
% !$m$    $\syneq$ get $m$
% $m$ ← $a$ $\syneq$ set $m$ $a$
%
% term sort-two (mx my : mutable integer) : unit
%   ≔ let x ≔ !mx in
%     let y ≔ !my in
%     if x > y
%       then mx ← y >> my ← x
%       else •.
%
% term list-sum (l : list integer) : integer
%   ≔ do
%       { let s : mutable integer ≔ initialize 0
%       ; let i : mutable integer ≔ initialize 0
%       ; while !i < length l
%           loop do
%             { let x : integer ≔ l[!i]
%             ; s ← !s + x
%             ; i ← !i + 1 }
%           done !s }.
% \end{snippet}

% ------------------------------------------------------------------------------
% Mona
% ------------------------------------------------------------------------------

% \begin{snippet}
% class Monad (M : kind → kind) : kind
%   { lift (α:kind)     : α → M α
%   ; map  (α β : kind) : (α → β) → M α → M β
%   ; bind (α β : kind) : M α → (α → M β) → M β }.
% \end{snippet}
%
% \begin{snippet}
% type nondeterministic : kind → kind ≔ list.
%
% instance Monad nondeterministic
%   { lift a   ≔ [a]
%   ; map  f m ≔ cases m
%                 { []     ⇒ []
%                 | a ∷ m' ⇒ f a ∷ map f m' }
%   ; bind m k ≔ concat (map k m) }.
%
% $m$ >>= $k$    $\syneq$    bind $m$ $k$
% $m$ >> $m'$    $\syneq$    bind $m$ (_ ⇒ $m$')
%
% term flip-coin : nondeterministic boolean ≔ [true, false].
%
% term lucky : nondeterministic boolean
%   ≔ flip-coin >>= (b1 ⇒
%       flip-coin >>= (b2 ⇒
%         lift (b1 ∧ b2))).
%
% term lucky : nondeterministic boolean
%   ≔ do
%       { let b1 ← flip-coin
%       ; let b2 ← flip-coin
%       ; lift (b1 ∧ b2) }.
% \end{snippet}
% \newpage
% \begin{snippet}
% lucky
% $↠$
% do{ let b1 ← [true, false]; let b2 ← [true, false]; lift (b1 ∧ b2) }
% $↠$
% flip-coin >>= (b1 ⇒ [true, false] >>= (b2 ⇒ lift (b1 ∧ b2)))
% $↠$ $\ruleappwith{Apply}{bind}$
% concat (map (b1 ⇒ [true, false] >>= (b2 ⇒ lift (b1 ∧ b2)))
%           [true, false])
% $↠$ $\ruleappwith{Apply}{bind}$
% concat (map (b1 ⇒
%               concat (map (b2 ⇒ lift (b1 ∧ b2))
%                         [true, false]))
%           [true, false])
% $↠$ $\ruleappwith{Apply}{lift}$
% concat (map (b1 ⇒
%               concat (map (b2 ⇒ [b1 ∧ b2])
%                         [true, false]))
%           [true, false])
% $↠$ $\ruleappwith{Apply}{map}$
% concat (map (b1 ⇒
%               [b1 ∧ true, b1 ∧ false])
%           [true, false])
% $↠$ $\ruleappwith{Apply}{map}$
% [true ∧ true, true ∧ false, false ∧ true, false ∧ false]
% $↠$
% [true, false, false, false]
% \end{snippet}

% \begin{snippet}
% type exceptional (ε α : kind) : kind
%   { throw : ε → exceptional ε α
%   | valid : α → exceptional ε α }.
%
% instance (ε:kind) ⇒ Monad (exceptional ε)
%   { lift a   ≔ valid a
%   ; map  f m ≔ cases m
%                 { throw e ⇒ throw e
%                 | valid a ⇒ valid (f a) }
%   ; bind m k ≔ cases m
%                 { throw e ⇒ throw e
%                 | valid a ⇒ k a } }.
%
% term divide-safely (r s : rational)
%   : exceptional rational rational
%   ≔ if s == 0
%       then throw r
%       else lift (r/s).
%
% term reciprocals-sum (r s : rational)
%   : exceptional rational rational
%   ≔ do
%       { let q  ← divide-safely r s
%       ; let q' ← divide-safely s r
%       ; lift (q + q') }.
% \end{snippet}

% ------------------------------------------------------------------------------
% Alge
% ------------------------------------------------------------------------------

% \begin{snippet}
% resource Coin { flip : unit ↗ boolean }.
%
% channel coin : Coin.
%
% term lucky : boolean
%   ≔ (coin#flip •) ∧ (coin#flip •).
%
% term either-heads-or-tails
%   : Coin → boolean ↘ list boolean
%   ≔ handler
%       { #flip _ k ⇒ k true ◇ k false
%       ; value x   ⇒ [x]
%       ; final l   ⇒ l }.
%
% lucky with either-heads-or-tails
% \end{snippet}

% \begin{snippet}
% h := either-heads-or-tails
%
% $[]$  ;  $[]$ $\|$ lucky with either-heads-or-tails
% $↠$
% $[]$  ; $[]$ $\|$ (coin#flip •) ∧ (coin#flip •) with either-heads-or-tails
% $↠$ $\ruleapp{Handle}$
% $[$h$]$ ; $[]$ $\|$ (coin#flip •) ∧ (coin#flip •)
% $↠$ $\ruleapp{Perform}$
% $[$h$]$ ; $[$(coin#flip •, $@_1$)$]$ $\|$ (coin#flip •) ∧ $@_1$
% $↠$ $\ruleapp{Perform}$
% $[$h$]$ ; $[$(coin#flip •, $@_2$), (coin#flip •, $@_1$)$]$ $\|$ $@_2$ ∧ $@_1$
% $↠$ $\ruleapp{Value}$
% $[$h$]$ ; $[$(coin#flip •, $@_2$), (coin#flip •, $@_1$)$]$ $\|$ [$@_2$ ∧ $@_1$]
% $↠$ $\ruleapp{Handle-Performance}$
% $[$h$]$ ; $[$(coin#flip •, $@_1$)$]$ $\|$ [true ∧ $@_1$] ◇ [false ∧ $@_1$]
% $↠$
% $[$h$]$ ; $[$(coin#flip •, $@_1$)$]$ $\|$ [true ∧ $@_1$, false ∧ $@_1$]
% $↠$ $\ruleapp{Handle-Performance}$
% $[$h$]$ ; $[]$ $\|$ [true ∧ true, false ∧ true] ◇ [true ∧ false, false ∧ false]
% $↠$
% $[$h$]$ ; $[]$ $\|$ [true, false, false, false]
% $↠$ $\ruleapp{Handle-Final}$
% $[]$  ; $[]$ $\|$ [true, false, false, false]
%
% ($@$ ⇒ $w$)
%
% \end{snippet}

% ------------------------------------------------------------------------------
% Frer
% ------------------------------------------------------------------------------

\begin{snippet}
instance (υ : kind → kind) ⇒ Monad (freer υ)
  { lift a   ≔ pure a
  ; map  f m ≔ cases m
                { pure   a   ⇒ pure (f a)
                | impure y q ⇒ impure y (map f ○ q) }
  ; bind m k ≔ cases m
                { pure   x   ⇒ k x
                | impure y q ⇒ impure y (x ⇒ bind (q x) k) } }.
\end{snippet}

\begin{snippet}
type nondeterministic-base : kind → kind ≔ list.
type nondeterministic      : kind → kind ≔ freer nondeterministic-base.

term sample-base (α:kind) (l : list α) : nondeterministic-base α ≔ l.
term sample      (α:kind) (l : list α) : freer-lift (sample-base l).

effect nondeterministic
 lifts list
  { sample l ≔ l }.
\end{snippet}

\begin{snippet}
type exceptional-base (ε α : kind) : kind ≔ ε ⊕ α.
type exceptional      (ε α : kind) : kind ≔ freer (exceptional-base ε) α.

term throw-base (ε α : kind) (e:ε) : exceptional-base ε α ≔ left e.
term throw-base (ε α : kind) (e:ε) : exceptional      ε α ≔ freer-lift (throw-base e).

term valid-base (ε α : kind) (a:α) : exceptional-base ε α ≔ right a.
term valid      (ε α : kind) (a:α) : exceptional      ε α ≔ freer-lift (valid-base a).
\end{snippet}

\end{document}
