\begin{table}[H] \centering
\captionof{table}{Typing in \LangA}
\begin{tabular}{rp{15em}}
  \rulename{Simple} &
  \code|$\jctx$, $a$:$α$ $⊢$ $a$:$α$|
\\[2em]
  \rulename{Simple} &
  \code|$\jctx$, $α$:$A$ $⊢$ $α$:$A$|
\\[2em]
  \rulename{Term-Abstraction} &
  \begin{tabular}{p{15em}}
    \code|$\jctx$, $a$:$α$ $⊢$ $b$:$β$|
    \\ \hline
    \code|$\jctx$ $⊢$ ($a$:$α$) ⇒ $b$ : $α$ → $β$|
  \end{tabular}
\\[2em]
  \rulename{Term-Application} &
  \begin{tabular}{p{15em}}
    \code|$\jctx$ $⊢$ $f$ : $α$ → $β$| \iand
    \code|$\jctx$ $⊢$ $a$:$α$|
    \\ \hline
    \code|$\jctx$ $⊢$ $f$ $a$ : $β$|
  \end{tabular}
\\[2em]
  \rulename{Type-Abstraction} &
  \begin{tabular}{p{15em}}
    \code|$\jctx$, $α$:$A$ $⊢$ $β$:$B$|
    \\ \hline
    \code|$\jctx$ $⊢$ ($α$:$A$) ⇒ $B$ : $A$ → $B$|
  \end{tabular}
\\[2em]
  \rulename{Type-Application} &
  \begin{tabular}{p{15em}}
    \code|$\jctx$ $⊢$ $φ$ : $Α$ → $Β$| \iand
    \code|$\jctx$ $⊢$ $α$:$Α$|
    \\ \hline
    \code|$\jctx$ $⊢$ $φ$ $α$ : $B$|
  \end{tabular}
\end{tabular}
\label{tab:LangA-typing}
\end{table}
